access: strengthen integrity_asids on RISCV64
Signed-off-by: Ryan Barry <ryan.barry@unsw.edu.au>

proof/access-control/RISCV64/ArchAccess.thy
@@ -117,36 +117,86 @@ section \<open>Arch-specific integrity definition\<close>
 
 subsection \<open>How ASIDs can change\<close>
 
-abbreviation integrity_asids_aux ::
-  "'a PAS \<Rightarrow> 'a set \<Rightarrow> asid \<Rightarrow> obj_ref option \<Rightarrow> obj_ref option \<Rightarrow> bool" where
-  "integrity_asids_aux aag subjects asid pp_opt pp_opt' \<equiv>
-     pp_opt = pp_opt' \<or> (\<forall>asid'. asid' \<noteq> 0 \<and> asid_high_bits_of asid' = asid_high_bits_of asid
-                                 \<longrightarrow> pasASIDAbs aag asid' \<in> subjects)"
+abbreviation integrity_asids_aux :: "'a PAS \<Rightarrow> 'a set \<Rightarrow> obj_ref \<Rightarrow> asid \<Rightarrow>
+                                     (asid_high_index \<rightharpoonup> obj_ref) \<Rightarrow> (asid_high_index \<rightharpoonup> obj_ref) \<Rightarrow>
+                                     (obj_ref \<rightharpoonup> asid_pool) \<Rightarrow> (obj_ref \<rightharpoonup> asid_pool) \<Rightarrow> bool" where
+  "integrity_asids_aux aag subjects x asid atab atab' pools pools'  \<equiv>
+     (atab (asid_high_bits_of asid) \<noteq> atab' (asid_high_bits_of asid)
+      \<longrightarrow> (\<forall>x. atab' (asid_high_bits_of asid) = Some x \<longrightarrow> pasObjectAbs aag x \<in> subjects) \<and>
+          (\<forall>asid'. asid' \<noteq> 0 \<and> asid_high_bits_of asid' = asid_high_bits_of asid
+                   \<longrightarrow> pasASIDAbs aag asid' \<in> subjects)) \<and>
+     (pasObjectAbs aag x \<notin> subjects
+      \<longrightarrow> (\<forall>pool. pools x = Some pool
+                  \<longrightarrow> pools' x \<noteq> None \<and>
+                      (\<forall>pool'. pools' x = Some pool' \<longrightarrow>
+                               (pool \<noteq> pool' \<longrightarrow> (\<exists>asid. atab (asid_high_bits_of asid) = Some x)))))"
 
 definition integrity_asids ::
-  "'a PAS \<Rightarrow> 'a set \<Rightarrow> asid \<Rightarrow> 'y::state_ext state \<Rightarrow> 'z:: state_ext state  \<Rightarrow> bool" where
-  "integrity_asids aag subjects x s s' \<equiv>
-   integrity_asids_aux aag subjects x (asid_table s  (asid_high_bits_of x))
-                                      (asid_table s' (asid_high_bits_of x))"
-
-declare integrity_asids_def[simp]
+  "'a PAS \<Rightarrow> 'a set \<Rightarrow> obj_ref \<Rightarrow> asid \<Rightarrow> 'y::state_ext state \<Rightarrow> 'z::state_ext state  \<Rightarrow> bool" where
+  "integrity_asids aag subjects x asid s s' \<equiv>
+   integrity_asids_aux aag subjects x asid (asid_table s) (asid_table s')
+                                           (asid_pools_of s) (asid_pools_of s')"
 
 sublocale kheap_update: Arch_arch_update_eq "kheap_update f"
   by unfold_locales simp
 
-lemma (in Arch_arch_update_eq) integrity_asids_update[simp]:
-  "integrity_asids aag subjects x (f st) s = integrity_asids aag subjects x st s"
-  "integrity_asids aag subjects x st (f s) = integrity_asids aag subjects x st s"
-  by (auto simp: arch)
+lemma (in Arch_p_arch_update_eq) integrity_asids_update[simp]:
+  "integrity_asids aag subjects x a (f st) s = integrity_asids aag subjects x a st s"
+  "integrity_asids aag subjects x a st (f s) = integrity_asids aag subjects x a st s"
+  by (auto simp: integrity_asids_def arch pspace)
 
 lemmas integrity_asids_updates =
   cdt_update.integrity_asids_update
   more_update.integrity_asids_update
-  kheap_update.integrity_asids_update
   revokable_update.integrity_asids_update
   interrupt_update.integrity_asids_update
   cur_thread_update.integrity_asids_update
   machine_state_update.integrity_asids_update
+
+lemma integrity_asids_cnode_update':
+  "\<lbrakk> kheap st p = Some (CNode sz cs); integrity_asids aag subjects x a st (s\<lparr>kheap := rest\<rparr>) \<rbrakk>
+     \<Longrightarrow> integrity_asids aag subjects x a st (s\<lparr>kheap := \<lambda>x. if x = p then v else rest x\<rparr>)"
+  by (auto simp: integrity_asids_def opt_map_def split: option.splits)
+
+lemma integrity_asids_tcb_update':
+  "\<lbrakk> kheap st p = Some (TCB tcb); integrity_asids aag subjects x a st (s\<lparr>kheap := rest\<rparr>) \<rbrakk>
+     \<Longrightarrow> integrity_asids aag subjects x a st (s\<lparr>kheap := \<lambda>x. if x = p then v else rest x\<rparr>)"
+  by (auto simp: integrity_asids_def opt_map_def split: option.splits)
+
+lemma integrity_asids_ep_update':
+  "\<lbrakk> kheap st p = Some (Endpoint ep); integrity_asids aag subjects x a st (s\<lparr>kheap := rest\<rparr>) \<rbrakk>
+     \<Longrightarrow> integrity_asids aag subjects x a st (s\<lparr>kheap := \<lambda>x. if x = p then v else rest x\<rparr>)"
+  by (auto simp: integrity_asids_def opt_map_def split: option.splits)
+
+lemma integrity_asids_ntfn_update':
+  "\<lbrakk> kheap st p = Some (Notification ntfn); integrity_asids aag subjects x a st (s\<lparr>kheap := rest\<rparr>) \<rbrakk>
+     \<Longrightarrow> integrity_asids aag subjects x a st (s\<lparr>kheap := \<lambda>x. if x = p then v else rest x\<rparr>)"
+  by (auto simp: integrity_asids_def opt_map_def split: option.splits)
+
+lemmas integrity_asids_kh_upds'' =
+  integrity_asids_cnode_update'
+  integrity_asids_tcb_update'
+  integrity_asids_ep_update'
+  integrity_asids_ntfn_update'
+
+lemmas integrity_asids_kh_upds =
+  integrity_asids_kh_upds''
+  integrity_asids_kh_upds''[where rest="kheap s" and s=s for s, folded fun_upd_def, simplified]
+
+declare integrity_asids_def[simp]
+
+lemma integrity_asids_kh_upds':
+  "integrity_asids aag subjects x a (s\<lparr>kheap := kheap s(p \<mapsto> CNode sz cs)\<rparr>) s"
+  "integrity_asids aag subjects x a (s\<lparr>kheap := kheap s(p \<mapsto> TCB tcb)\<rparr>) s"
+  "integrity_asids aag subjects x a (s\<lparr>kheap := kheap s(p \<mapsto> Endpoint ep)\<rparr>) s"
+  "integrity_asids aag subjects x a (s\<lparr>kheap := kheap s(p \<mapsto> Notification ntfn)\<rparr>) s"
+  by (auto simp: opt_map_def split: option.splits)
+
+lemma integrity_asids_kh_update:
+  "integrity_asids aag subject x a (s\<lparr>kheap := kh\<rparr>) (s\<lparr>kheap := kh'\<rparr>)
+   \<Longrightarrow> integrity_asids aag subject x a (s\<lparr>kheap := kh(p := v)\<rparr>) (s\<lparr>kheap := kh'(p := v)\<rparr>)"
+  by (clarsimp simp: opt_map_def)
+
 
 subsection \<open>Misc definitions\<close>
 
@@ -216,6 +266,9 @@ requalify_consts
 requalify_facts
   integrity_asids_updates
   state_vrefs_upd
+  integrity_asids_kh_upds
+  integrity_asids_kh_upds'
+  integrity_asids_kh_update
 
 end
 
