proof/access-control/Finalise_AC.thy
@@ -414,7 +414,7 @@ lemma sbn_unbind_respects[wp]:
   apply (simp add: set_bound_notification_def)
   apply (wpsimp wp: set_object_wp)
   apply (erule integrity_trans)
-  apply (clarsimp simp: integrity_def obj_at_def pred_tcb_at_def)
+  apply (clarsimp simp: integrity_def obj_at_def pred_tcb_at_def integrity_asids_kh_upds)
   apply (rule tro_tcb_unbind)
      apply (fastforce dest!: get_tcb_SomeD)
     apply (fastforce dest!: get_tcb_SomeD)
